\documentclass[12 pt letterpaper]{article}
\usepackage{amsmath,amssymb,amscd,amsthm,amsxtra}
\usepackage{latexsym}
\usepackage[dvips]{graphics,epsfig}
%\usepackage{graphicx}

\setlength{\topmargin}{-0.5in}
\setlength{\oddsidemargin}{0in}
\setlength{\evensidemargin}{0in}
\setlength{\textwidth}{6.5in}


%\headheight=8pt
%\topmargin=0pt
\textheight=624pt
%\textwidth=432pt
%\oddsidemargin=18pt
%\evensidemargin=18pt

\newcommand{\LA}{\Longrightarrow}

\pagestyle{empty}
%\setlength{\voffset}{-1cm}
%\setlength{\hoffset}{-1.6cm}
%\setlength{\oddsidemargin }{0cm}
%\setlength{\textwidth}{15cm}



\begin{document}


\large
\begin{center}
\textbf{MATH331: Solution to the Last Homework}
\end{center}
\vspace{0.6cm}

\normalsize

\noindent {\bf \underline{6.2}}

\noindent
1. 
\[F(s) = \frac{3}{s^2+4} = \frac{3}{2} \frac{2}{s^2 +2^2}
\Longrightarrow f(t) = \frac{3}{2} \sin 2t.\]

\noindent
3. \[F(s) = \frac{2}{s^2 + 3s - 4} = \frac{2}{(s + 4)(s - 1)}
= \frac{2}{5}\frac{1}{s-1} - \frac{2}{5}\frac{1}{s-(-4)}
\Longrightarrow f(t) = \frac{2}{5} e^t -\frac{2}{5} e^{-4t}.\]

\noindent
4. \[F(s) = \frac{3s}{s^2 - s- 6} = \frac{3s}{(s-3)(s+2)}
= \frac{6}{5} \frac{1}{s+2} + \frac{9}{5}\frac{1}{s-3}
\Longrightarrow f(t) = \frac{6}{5} e^{-2t} + \frac{9}{5} e^{3t}.\]

\noindent
5. \[F(s) = \frac{2s + 2}{s^2 +2s+5} = \frac{2(s+1)}{(s+1)^2 +2^2}
\Longrightarrow f(t) = 2 e^{-t}\cos 2t. \]

\noindent
6. \[F(s) = \frac{2s-3}{s^2 -4} = \frac{2s -3}{(s+2)(s-2)}
= \frac{7}{4}\frac{1}{s+2} + \frac{1}{4}\frac{1}{s-2}
\Longrightarrow f(t) = \frac{7}{4} e^{-2t} + \frac{1}{4} e^{2t}.\]
NOTE: This can be written as $2 \cosh 2t - \frac{3}{2} \sinh2t$
since $\cosh x = \frac{e^x + e^{-x}}{2}$ and 
$\sinh x = \frac{e^x - e^{-x}}{2}$.

\noindent
8. \[F(s) = \frac{8 s^2 - 4s + 12}{s(s^2+4)} = \frac{5s-4}{s^2+4} + \frac{3}{s}
= 5\frac{s}{s^2+2^2} -2\frac{2}{s^2 + 2^2} +3\frac{1}{s} 
\Longrightarrow f(t) = 5 \cos 2t -2 \sin 2t +3. \]

\noindent
13. By taking the Laplace transform of the ODE, we have
\begin{gather*} s^2 Y(s) -s \cdot 0 - 1 -2(sY(s) - 0) + 2 Y(s) = 0
\Longrightarrow (s^2 -2s + 2) Y(s) = 1 \\
\LA Y(s) = \frac{1}{s^2 -2s + 2} = \frac{1}{(s-1)^2 +1^2}
\LA y(t) = e^t \sin t.  
\end{gather*}

\noindent
14. By taking the Laplace transform of the ODE, we have
\begin{gather*} s^2 Y(s) -s \cdot 1 - 1 -4(sY(s) - 1) + 4Y(s) = 0
\LA (s^2 -4s +4) Y(s) = s -3 \\
\LA  Y(s) = \frac{s-2 -1}{(s-2)^2} = \frac{1}{s-2} - \frac{1}{(s-2)^2}
\LA y(t) = e^{2t} - te^{2t}. 
\end{gather*}

\noindent
20. By taking the Laplace transform of the ODE, we have
\begin{gather*} s^2 Y(s) -s \cdot 1 - 0  + \omega^2 Y(s) = \frac{s}{s^2+4}
\LA  (s^2 +\omega^2) Y(s) = \frac{s}{s^2+4} +s \\
\LA Y(s) = \frac{s}{(s^2+4)(s^2 +\omega^2)} + \frac{s}{s^2 +\omega^2}
= \frac{1}{\omega^2 - 4} \frac{s}{s^2+2^2} - \frac{1}{\omega^2 - 4} \frac{s}{s^2+\omega^2}
+ \frac{s}{s^2 +\omega^2} \\
\LA y(t) = \frac{1}{\omega^2 - 4} \cos 2t - \frac{1}{\omega^2 - 4} \cos \omega t
+ \cos \omega t
= \frac{1}{\omega^2 - 4} \cos 2t + \frac{\omega^2 - 5}{\omega^2 - 4} \cos \omega t.
\end{gather*}

\noindent
22. By taking the Laplace transform of the ODE, we have
\begin{gather*} s^2 Y(s) -s \cdot 0 - 1 -2(sY(s) - 0) + 2Y(s) = \frac{1}{s+1}
\LA (s^2 -2s +2) Y(s) = \frac{1}{s+1} +1 \\
\LA Y(s) = \frac{1}{(s+1)\big( (s-1)^2 + 1\big)} + \frac{1}{(s-1)^2+1} 
= \frac{1}{5}\frac{1}{s+1} -\frac{1}{5} \frac{s-3}{(s-1)^2 + 1} + \frac{1}{(s-1)^2+1}\\
= \frac{1}{5}\frac{1}{s+1} -\frac{1}{5} \frac{s-1}{(s-1)^2 + 1} + \frac{7}{5}\frac{1}{(s-1)^2+1}
\LA y(t) = \frac{1}{5} e^{-t} - \frac{1}{5} e^t \cos t + \frac{7}{5} e^t \sin t.
\end{gather*}

\noindent
23. By taking the Laplace transform of the ODE, we have
\begin{gather*} s^2 Y(s) -s \cdot 2 -(- 1) + 2(sY(s) - 2) + Y(s) = \frac{4}{s+1}
\LA (s^2 + 2s + 1) Y(s) = \frac{4}{s+1} + 2s + 3\\
\LA Y(s) = \frac{4}{(s+1)^3} + \frac{2(s+1) + 1}{(s+1)^2}
= 2 \frac{2 \! }{(s+1)^3} + \frac{2}{s+1} + \frac{1}{(s+1)^2}
\LA y(t) = 2 t^2 e^{-t} + 2 e^{-t} + t e^{-t}.
\end{gather*}

\vspace{2mm}

\noindent {\bf \underline{6.3}}

\noindent
7. \[f(t) = u_2(t)(t-2)^2  \LA F(s) = e^{-2s} \frac{2}{s^3}.\]

\noindent
9. \[f(t) = \big(u_\pi (t) - u_{2\pi}(t) \big) (t- \pi)
= u_\pi(t) (t- \pi) - u_{2\pi}(t - 2 \pi) - \pi u_{2\pi}
\LA F(s) = \frac{e^{-\pi s}}{s^2} - \frac{e^{-2\pi s}}{s^2} - \frac{\pi e^{-2\pi s}}{s}.\]

\noindent
14.
\[F(s) = e^{-2s}\frac{1}{(s+2)(s - 1)} 
= e^{-2s} \left( \frac{1}{3} \frac {1}{s- 1} - \frac{1}{3} \frac{1}{s+2} \right)
\LA f(t) = \frac{1}{3}u_2(t) e^{t- 2} - \frac{1}{3} u_2(t) e^{-2(t-2)} .
\]

\noindent
15.
\[F(s) = e^{-2s} \frac{2(s-1)}{(s-1)^2 + 1^2}
\LA f(t) = 2 u_2(t) e^{(t-2)} \cos (t- 2).\]

\noindent
16.
\[F(s) = 2 e^{-2s} \frac{1}{(s+2)(s-2)} 
= 2 e^{-2s} \frac{1}{4} \left(\frac{1}{s-2} - \frac{1}{s+2} \right) 
\LA f(t) =  \frac{1}{2}u_2(t) \big( e^{2(t-2)} - e^{-2(t-2)}\big)
= u_2(t) \sinh 2(t-2).\]


\vspace{2mm}

\noindent {\bf \underline{6.4}}

\noindent
3. By taking the Laplace transform of the ODE, we have
\begin{gather*} s^2 Y(s) -s \cdot 0 - 0  + 4 Y(s) 
= \frac{1}{s^2+1} - e^{-2\pi t}\frac{1}{s^2+1}\\
\LA Y(s) = (1 - e^{-2\pi t}) \frac{1}{s^2+4}\frac{1}{s^2+1}
= (1 - e^{-2\pi t}) \frac{1}{3} \left( \frac{1}{s^2+1}- \frac{1}{s^2+4} \right)\\
\LA y(t) = \frac{1}{3}(\sin t - \frac{1}{2} \sin 2t)
- \frac{1}{3}u_{2 \pi}(t) (\sin (t-2\pi) - \frac{1}{2} \sin 2(t-2\pi))
= \frac{1}{3}\big( 1 - u_{2\pi}(t)\big) (\sin t - \frac{1}{2} \sin 2t),
\end{gather*}
because $\sin (t-2\pi) = \sin t$ and $\sin 2(t-2\pi) = \sin 2t$.

\noindent
4. By taking the Laplace transform of the ODE, we have
\begin{gather*} s^2 Y(s) -s \cdot 0 - 0  + 4 Y(s) 
= \frac{1}{s^2+1} + e^{-\pi t}\frac{1}{s^2+1}\\
\LA Y(s) = (1 + e^{-\pi t}) \frac{1}{s^2+4}\frac{1}{s^2+1}
= (1 + e^{-\pi t}) \frac{1}{3} \left( \frac{1}{s^2+1}- \frac{1}{s^2+4} \right)\\
\LA y(t) = \frac{1}{3}(\sin t - \frac{1}{2} \sin 2t)
+ \frac{1}{3}u_{ \pi}(t) (\sin (t-\pi) - \frac{1}{2} \sin 2(t-\pi))
= \frac{1}{3}\big( 1 - u_{\pi}(t)\big) \sin t 
- \frac{1}{6}\big( 1 + u_{\pi}(t)\big) \sin 2t,
\end{gather*}
because $\sin (t-\pi) = -\sin t$ and $\sin 2(t-\pi) = \sin 2t$.

\noindent
7. By taking the Laplace transform of the ODE, we have
\begin{gather*} s^2 Y(s) -s \cdot 1 - 0  +  Y(s) 
= \frac{e^{-3\pi s}}{s} 
\LA Y(s) = \frac{e^{-3\pi s}}{s(s^2+1)} + \frac{s}{s^2+1}
= e^{-3\pi s} \left(\frac{1}{s} - \frac{s}{s^2+1} \right) + \frac{s}{s^2+1}\\
\LA y(t) = u_{3 \pi}(t) \big(1 - \cos (t- 3 \pi) \big) + \cos t.
\end{gather*}


%\Longrightarrow 
\end{document}